BasicTypingProp.v
@@ -1,121 +1,177 @@
 From stdpp Require Import mapset.
-From CT Require Import CoreLangProp.
+From CT.Syntax Require Import Syntax.
 From CT Require Import BasicTyping.
 From CT Require Import OperationalSemantics.
 
-Import Atom.
-Import CoreLang.
-Import Tactics.
-Import NamelessTactics.
+Import BaseDef MyTactics Primitives Lang Lc.
+Import LangLc.
 Import BasicTyping.
 Import OperationalSemantics.
 
+(* NOTE:
+   Using [change ... in *] with shared evars (the [?Γ ?e ?T] placeholders)
+   often fails when there are multiple [value_has_type]/[tm_has_type]
+   occurrences with different parameters in the context/goal.
+   We instead rewrite each occurrence one-by-one by first pattern-matching to
+   bind fresh [Γ e T] for that specific occurrence. *)
+Ltac fold_typing_class :=
+  change (value_has_type ?Γ ?v ?T) with (Γ ⊢ v ⋮ T) in *;
+  change (tm_has_type ?Γ ?e ?T) with (Γ ⊢ e ⋮ T) in *;
+  repeat (
+    first
+      [ progress match goal with
+        | H : context [value_has_type ?Γ ?v ?T] |- _ =>
+            change (value_has_type Γ v T) with (Γ ⊢ v ⋮ T) in H
+        | |- context [value_has_type ?Γ ?v ?T] =>
+            change (value_has_type Γ v T) with (Γ ⊢ v ⋮ T)
+        end
+      | progress match goal with
+        | H : context [tm_has_type ?Γ ?e ?T] |- _ =>
+            change (tm_has_type Γ e T) with (Γ ⊢ e ⋮ T) in H
+        | |- context [tm_has_type ?Γ ?e ?T] =>
+            change (tm_has_type Γ e T) with (Γ ⊢ e ⋮ T)
+        end
+      ]).
+
 (** * Naming related properties of the basic type system *)
 
-Lemma basic_typing_contains_fv_tm: forall Γ e T, Γ ⊢t e ⋮t T -> fv_tm e ⊆ dom Γ
-with basic_typing_contains_fv_value: forall Γ e T, Γ ⊢t e ⋮v T -> fv_value e ⊆ dom Γ.
+Lemma basic_typing_contains_fv_tm: forall Γ (e: tm) T, Γ ⊢ e ⋮ T -> stale e ⊆ dom Γ
+with basic_typing_contains_fv_value: forall Γ (e: value) T, Γ ⊢ e ⋮ T -> stale e ⊆ dom Γ.
 Proof.
   all:
   destruct 1; simpl; eauto;
   try select (forall x, _ ∉ _ -> _) (fun H => auto_pose_fv x; repeat specialize_with x);
-  repeat select (_ ⊢t _ ⋮v _) (fun H => apply basic_typing_contains_fv_value in H);
-  repeat select (_ ⊢t _ ⋮t _) (fun H => apply basic_typing_contains_fv_tm in H);
-  simpl in *;
+  repeat select (tm_has_type _ _ _) (fun H => apply basic_typing_contains_fv_tm in H);
+  repeat select (value_has_type _ _ _) (fun H => apply basic_typing_contains_fv_value in H);
+  ln_simpl;
   repeat
     match goal with
-    | H : fv_tm ({_ ~t> _} _) ⊆ _ |- _ =>
-        setoid_rewrite <- open_fv_tm' in H
-    | H : _ ⊆ dom (<[_:=_]>_) |- _ =>
+    | H : stale ({_ ~> _} _) ⊆ _ |- _ ⊆ _ =>
+        setoid_rewrite <- open_fv' in H
+    | H : _ ⊆ dom (<[_:=_]>_) |- _ ⊆ _ =>
         setoid_rewrite dom_insert in H
-    | H : _ !! _ = _ |- _ =>
-        apply elem_of_dom_2 in H
+    | H : _ !! _ = _ |- _ ⊆ _ =>
+        apply elem_of_dom_2 in H; simp_hyps
     end;
   my_set_solver.
 Qed.
 
-Lemma basic_typing_closed_tm: forall e T, ∅ ⊢t e ⋮t T -> closed_tm e.
+Class FvSubsetGamma (G E T: Type) `{staleG: Stale G} `{staleE: Stale E} `{Typing G E T} := fv_subset_gamma: forall (Γ: G) (e: E) (T: T), Γ ⊢ e ⋮ T -> staleE e ⊆ staleG Γ.
+
+#[global] Instance FvSubsetGamma_tm: FvSubsetGamma tyctx tm ty.
+Proof.
+  unfold FvSubsetGamma.
+  eapply basic_typing_contains_fv_tm; eauto.
+Qed.
+Arguments FvSubsetGamma_tm /.
+
+#[global] Instance FvSubsetGamma_value: FvSubsetGamma tyctx value ty.
+Proof.
+  unfold FvSubsetGamma.
+  eapply basic_typing_contains_fv_value; eauto.
+Qed.
+Arguments FvSubsetGamma_value /.
+
+Lemma basic_typing_closed_tm: forall e T, ∅ ⊢ e ⋮ T -> stale e ≡ ∅.
 Proof.
   intros.
-  apply basic_typing_contains_fv_tm in H. my_set_solver.
+  apply fv_subset_gamma in H. my_set_solver.
 Qed.
 
-Lemma basic_typing_closed_value: forall v T, ∅ ⊢t v ⋮v T -> closed_value v.
+Lemma basic_typing_closed_value: forall v T, ∅ ⊢ v ⋮ T -> stale v ≡ ∅.
 Proof.
   intros.
-  apply basic_typing_contains_fv_value in H. my_set_solver.
+  apply fv_subset_gamma in H. my_set_solver.
 Qed.
 
-Lemma basic_typing_regular_value: forall Γ v t, Γ ⊢t v ⋮v t -> lc v
-with basic_typing_regular_tm: forall Γ e t, Γ ⊢t e ⋮t t -> lc e.
+Lemma basic_typing_regular_value: forall Γ (v: value) t, Γ ⊢ v ⋮ t -> lc v
+with basic_typing_regular_tm: forall Γ (e: tm) t, Γ ⊢ e ⋮ t -> lc e.
 Proof.
-  all: destruct 1; simpl;
-    try econstructor; try instantiate_atom_listctx; eauto.
+  all: destruct 1; ln_simpl; lc_solver;
+  try solve [try (auto_exists_L; intros y Hy; specialize_with y);
+  repeat match goal with
+  | [H: tm_has_type _ _ _ |- lc _] => apply basic_typing_regular_tm in H
+  | [H: value_has_type _ _ _ |- lc _] => apply basic_typing_regular_value in H
+  | [H: _ ⊢ ?e ⋮ _ |- lc _] =>
+    lazymatch type of e with
+    | tm => apply basic_typing_regular_tm in H
+    | value => apply basic_typing_regular_value in H
+    end
+  end; lc_solver].
 Qed.
+
+Class TypingLc (G E T: Type) `{Lc E} `{Typing G E T}  := typing_lc: forall (Γ: G) (e: E) (T: T), Γ ⊢ e ⋮ T -> lc e.
+
+#[global] Instance TypingLc_tm: TypingLc tyctx tm ty.
+Proof.
+  unfold TypingLc.
+  eapply basic_typing_regular_tm; eauto.
+Qed.
+Arguments TypingLc_tm /.
+
+#[global] Instance TypingLc_value: TypingLc tyctx value ty.
+Proof.
+  unfold TypingLc.
+  eapply basic_typing_regular_value; eauto.
+Qed.
+Arguments TypingLc_value /.
 
 Ltac lc_basic_typing_simp_aux :=
   match goal with
-  | [H: _ ⊢t ?e ⋮t _ |- lc ?e] => apply basic_typing_regular_tm in H
-  | [H: _ ⊢t ?v ⋮v _ |- lc (treturn ?v)] => apply basic_typing_regular_value in H
-  | [H: _ ⊢t _ ⋮v _ |- lc _] => apply basic_typing_regular_value in H; simp_hyps
-  | [H: _ ⊢t _ ⋮t _ |- lc _] => apply basic_typing_regular_tm in H; simp_hyps
-  | [H: _ ⊢t _ ⋮v _ |- body _] => apply basic_typing_regular_value in H; simp_hyps
-  | [H: _ ⊢t _ ⋮t _ |- body _] => apply basic_typing_regular_tm in H; simp_hyps
-  | [H: _ ⊢t _ ⋮v _ |- context [fv_value _]] =>
-      apply basic_typing_closed_value in H; simp_hyps
-  | [H: _ ⊢t _ ⋮t _ |- context [fv_value _]] =>
-      apply basic_typing_closed_tm in H; simp_hyps
-  | [H: _ ⊢t _ ⋮v _ |- context [fv_tm _]] =>
-      apply basic_typing_closed_value in H; simp_hyps
-  | [H: _ ⊢t _ ⋮t _ |- context [fv_tm _]] =>
-      apply basic_typing_closed_tm in H; simp_hyps
-  end; eauto.
+  | [H: _ ⊢ _ ⋮ _ |- lc _] => apply typing_lc in H
+  | [H: _ ⊢ _ ⋮ _ |- body _] => apply typing_lc in H
+  | [H: _ ⊢ _ ⋮ _ |- context [stale _]] => apply fv_subset_gamma in H
+  end.
 
 Ltac basic_typing_regular_simp :=
   repeat lc_basic_typing_simp_aux; eauto.
-
 
 (** This file proves properties of the basic type system. *)
 
 (** * Canonical forms *)
 
-Lemma basic_typing_bool_canonical_form: forall (v: value), ∅ ⊢t v ⋮v TBool -> v = true \/ v = false.
+Lemma basic_typing_bool_canonical_form: forall (v: value), ∅ ⊢ v ⋮ (TBase TBool) -> v = (vconst true) \/ v = (vconst false).
 Proof.
   inversion 1; subst; simpl in *.
   destruct c; simplify_eq. destruct b; eauto.
   simplify_map_eq.
 Qed.
 
-Lemma basic_typing_nat_canonical_form: forall (v: value), ∅ ⊢t v ⋮v TNat -> (exists (i: nat), v = i).
+Lemma basic_typing_nat_canonical_form: forall (v: value), ∅ ⊢ v ⋮ (TBase TNat) -> (exists (i: nat), v = vconst (cnat i)).
 Proof.
   inversion 1; subst; simpl in *.
   destruct c; simplify_eq. eauto.
   simplify_map_eq.
 Qed.
 
-Lemma basic_typing_base_canonical_form: forall (v: value) (B: base_ty), ∅ ⊢t v ⋮v B -> (exists (c: constant), v = c).
+Lemma basic_typing_base_canonical_form: forall (v: value) (B: base_ty), ∅ ⊢ v ⋮ (TBase B) -> (exists (c: constant), v = vconst c).
 Proof.
   inversion 1; subst. eauto. simplify_map_eq.
 Qed.
 
 Lemma basic_typing_arrow_canonical_form:
-  forall (v: value) T1 T2, ∅ ⊢t v ⋮v T1 ⤍ T2 ->
-                      (exists e, v = vlam T1 e) \/ (exists e, v = vfix (T1 ⤍ T2) (vlam (T1 ⤍ T2) e)).
+  forall (v: value) T1 T2, ∅ ⊢ v ⋮ T1 ⤍ T2 ->
+                      (exists e, v = vlam T1 e) \/ (exists e, v = vfix (T1 ⤍ T2) (treturn (vlam (T1 ⤍ T2) e))).
 Proof.
   inversion 1; subst. simplify_map_eq.
   - left. eauto.
   - right. eexists. f_equal.
 Qed.
 
-
 (** * Weakening lemmas *)
 
 Lemma basic_typing_weaken_tm: forall Γ Γ' (v: tm) T,
-    Γ ⊆ Γ' -> Γ ⊢t v ⋮t T -> Γ' ⊢t v ⋮t T
+    Γ ⊆ Γ' -> Γ ⊢ v ⋮ T -> Γ' ⊢ v ⋮ T
 with basic_typing_weaken_value: forall Γ Γ' (v: value) T,
-    Γ ⊆ Γ' -> Γ ⊢t v ⋮v T -> Γ' ⊢t v ⋮v T.
+    Γ ⊆ Γ' -> Γ ⊢ v ⋮ T -> Γ' ⊢ v ⋮ T.
 Proof.
-  all : intros * Hs; destruct 1; econstructor; eauto using lookup_weaken.
-  all: instantiate_atom_listctx;
+  all : intros * Hs; destruct 1;
+  try solve [econstructor; eauto using lookup_weaken].
+  all:
+    auto_exists_L; eauto;
+    fold_typing_class;
+  eauto;
+    intros x Hx; specialize_with x;
     auto_eapply;
     try lazymatch goal with
       | |- _ ⊆ _ => apply insert_mono; eauto
@@ -123,169 +179,309 @@ Proof.
       end.
 Qed.
 
-Lemma basic_typing_weaken_insert_tm: forall Γ (v: tm) T x U,
-    x # Γ -> Γ ⊢t v ⋮t T -> <[x := U]>Γ ⊢t v ⋮t T.
+Class BasicTypingWeaken (E: Type) `{Typing tyctx E ty} := basic_typing_weaken: forall (Γ Γ': tyctx) (e: E) (T: ty), Γ ⊆ Γ' -> Γ ⊢ e ⋮ T -> Γ' ⊢ e ⋮ T.
+
+#[global] Instance BasicTypingWeaken_tm: BasicTypingWeaken tm.
 Proof.
+  unfold BasicTypingWeaken.
+  eapply basic_typing_weaken_tm; eauto.
+Qed.
+Arguments BasicTypingWeaken_tm /.
+
+#[global] Instance BasicTypingWeaken_value: BasicTypingWeaken value.
+Proof.
+  unfold BasicTypingWeaken.
+  eapply basic_typing_weaken_value; eauto.
+Qed.
+Arguments BasicTypingWeaken_value /.
+
+Class BasicTypingWeakenInsert (E: Type) `{Typing tyctx E ty} := basic_typing_weaken_insert: forall (Γ: tyctx) (e: E) (T: ty) (x: atom) (U: ty), x # Γ -> Γ ⊢ e ⋮ T -> <[x := U]> Γ ⊢ e ⋮ T.
+
+#[global] Instance BasicTypingWeakenInsert_tm: BasicTypingWeakenInsert tm.
+Proof.
+  unfold BasicTypingWeakenInsert.
   intros. eapply basic_typing_weaken_tm. 2: eauto.
   apply insert_subseteq. apply not_elem_of_dom. my_set_solver.
 Qed.
+Arguments BasicTypingWeakenInsert_tm /.
 
-Lemma basic_typing_weaken_insert_value: forall Γ (v: value) T x U,
-    x # Γ -> Γ ⊢t v ⋮v T -> <[x := U]> Γ ⊢t v ⋮v T.
+#[global] Instance BasicTypingWeakenInsert_value: BasicTypingWeakenInsert value.
 Proof.
+  unfold BasicTypingWeakenInsert.
   intros. eapply basic_typing_weaken_value. 2: eauto.
   apply insert_subseteq. apply not_elem_of_dom. my_set_solver.
 Qed.
+Arguments BasicTypingWeakenInsert_value /.
 
 (** * Substitution lemmas *)
 
-Lemma basic_typing_subst_tm: forall Γ z u U (v: tm) T, Γ ⊢t u ⋮v U -> <[z := U]> Γ ⊢t v ⋮t T -> Γ ⊢t {z := u}t v ⋮t T.
+Class BasicTypingSubst (E: Type) `{Typing tyctx E ty} `{Subst value E} := basic_typing_subst: forall (Γ: tyctx) (z: atom) (u: value) (U: ty) (e: E) (T: ty), Γ ⊢ u ⋮ U -> <[z := U]> Γ ⊢ e ⋮ T -> Γ ⊢ {z := u} e ⋮ T.
+
+#[global] Instance BasicTypingSubst_tm: BasicTypingSubst tm.
 Proof.
+  unfold BasicTypingSubst.
   intros * Hu Ht; remember (<[z:=U]> Γ) as Γ'; generalize dependent Γ.
-  revert Γ' v T Ht.
+  revert Γ' e T Ht.
   apply (tm_has_type_mutual_rec
-           (fun c v T _ => ∀ Γ, Γ ⊢t u ⋮v U → c = <[z:=U]> Γ → Γ ⊢t {z := u }v v ⋮v T)
-           (fun c v T _ => ∀ Γ, Γ ⊢t u ⋮v U → c = <[z:=U]> Γ → Γ ⊢t {z := u }t v ⋮t T));
+           (fun c e T _ => ∀ Γ, Γ ⊢ u ⋮ U → c = <[z:=U]> Γ → Γ ⊢ {z := u } e ⋮ T)
+           (fun c e T _ => ∀ Γ, Γ ⊢ u ⋮ U → c = <[z:=U]> Γ → Γ ⊢ {z := u } e ⋮ T));
   (* [context] should be defined as a notation which helps resolving typeclass
   instances for, e.g., rewriting. *)
-    unfold context;
-    intros; subst; simpl in *; eauto; try econstructor; eauto.
-  case_decide; subst.
-  by simplify_map_eq.
-  econstructor. by simplify_map_eq.
-
-  all:
-  instantiate_atom_listctx;
-  rewrite <- subst_open_var_tm by
-    (eauto using basic_typing_regular_value; my_set_solver);
-  auto_eapply; [
-      eapply basic_typing_weaken_insert_value; eauto; my_set_solver
-    | apply insert_commute; my_set_solver ].
+    unfold tyctx;
+    intros; subst; ln_simpl; simplify_map_eq; eauto; try auto_exists_L; intros x Hx; specialize_with x; eauto;
+    ln_simpl;
+    fold_syntax_class; 
+    fold_typing_class;
+    eauto.
+  all: rewrite <- subst_open_var;
+  try match goal with
+  | [ |- _ ≠ _ ] => my_set_solver
+  | [H: _ ⊢ ?e ⋮ _ |- lc ?e ] => apply typing_lc in H; eauto
+  end; auto_eapply; fold_typing_class;
+  try match goal with
+  | [|- _ ∉ _ ] => my_set_solver
+  | [|- _ ⊢ _ ⋮ _ ] => eapply basic_typing_weaken_insert; eauto; my_set_solver
+  | _ => apply insert_commute; my_set_solver 
+  end.
 Qed.
+Arguments BasicTypingSubst_tm /.
 
-Lemma basic_typing_subst_value: forall Γ z u U (v: value) T, Γ ⊢t u ⋮v U -> <[z := U]> Γ ⊢t v ⋮v T -> Γ ⊢t {z := u}v v ⋮v T.
+#[global] Instance BasicTypingSubst_value: BasicTypingSubst value.
 Proof.
+  unfold BasicTypingSubst.
   intros * Hu Ht; remember (<[z:=U]> Γ) as Γ'; generalize dependent Γ.
-  revert Γ' v T Ht.
+  revert Γ' e T Ht.
   apply (value_has_type_mutual_rec
-           (fun c v T _ => ∀ Γ, Γ ⊢t u ⋮v U → c = <[z:=U]> Γ → Γ ⊢t {z := u }v v ⋮v T)
-           (fun c v T _ => ∀ Γ, Γ ⊢t u ⋮v U → c = <[z:=U]> Γ → Γ ⊢t {z := u }t v ⋮t T));
-    unfold context;
-    intros; subst; simpl in *; eauto; try econstructor; eauto.
-  case_decide; subst.
-  by simplify_map_eq.
-  econstructor. by simplify_map_eq.
-
-  all:
-  instantiate_atom_listctx;
-  rewrite <- subst_open_var_tm by
-    (eauto using basic_typing_regular_value; my_set_solver);
-  auto_eapply; [
-      eapply basic_typing_weaken_insert_value; eauto; my_set_solver
-    | apply insert_commute; my_set_solver ].
+           (fun c e T _ => ∀ Γ, Γ ⊢ u ⋮ U → c = <[z:=U]> Γ → Γ ⊢ {z := u } e ⋮ T)
+           (fun c e T _ => ∀ Γ, Γ ⊢ u ⋮ U → c = <[z:=U]> Γ → Γ ⊢ {z := u } e ⋮ T));
+  unfold tyctx;
+  intros; subst; ln_simpl; simplify_map_eq; eauto; try auto_exists_L; intros x Hx; specialize_with x; eauto;
+  ln_simpl;
+  fold_syntax_class; 
+  fold_typing_class;
+    eauto.
+  all: rewrite <- subst_open_var;
+  try match goal with
+  | [ |- _ ≠ _ ] => my_set_solver
+  | [H: _ ⊢ ?e ⋮ _ |- lc ?e ] => apply typing_lc in H; eauto
+  end; auto_eapply; fold_typing_class;
+  try match goal with
+  | [|- _ ∉ _ ] => my_set_solver
+  | [|- _ ⊢ _ ⋮ _ ] => eapply basic_typing_weaken_insert; eauto; my_set_solver
+  | _ => apply insert_commute; my_set_solver 
+  end.
 Qed.
+Arguments BasicTypingSubst_value /.
+
+Ltac smart_ln_simpl :=
+repeat match goal with
+| [H: lc ?e |- context [{_ ~> _} ?e]] => rewrite open_rec_lc by eauto
+| [H: lc ?e, H': context [{_ ~> _} ?e] |- _ ] => rewrite open_rec_lc in H' by eauto
+end.
+
+Class BasicTypingOpen (E: Type) `{Stale E} `{Typing tyctx E ty} `{Open value E} := basic_typing_open: forall (Γ: tyctx) (z: atom) (u: value) (U: ty) (e: E) (T: ty), z # e -> Γ ⊢ u ⋮ U -> <[z := U]> Γ ⊢ e ^^ (vfvar z) ⋮ T -> Γ ⊢ e ^^ u ⋮ T.
+
+#[global] Instance BasicTypingOpen_tm: BasicTypingOpen tm.
+Proof.
+  unfold BasicTypingOpen.
+  intros. rewrite <- subst_intro with (x:=z); eauto.
+  eapply basic_typing_subst in H1; eauto.
+  basic_typing_regular_simp.
+Qed.
+Arguments BasicTypingOpen_tm /.
+
+#[global] Instance BasicTypingOpen_value: BasicTypingOpen value.
+Proof.
+  unfold BasicTypingOpen.
+  intros. rewrite <- subst_intro with (x:=z); eauto.
+  eapply basic_typing_subst in H1; eauto.
+  basic_typing_regular_simp.
+Qed.
+Arguments BasicTypingOpen_value /.
 
 (** * Type uniqueness lemmas *)
 
-Lemma basic_typing_tm_unique: forall Γ e T1 T2,
-    Γ ⊢t e ⋮t T1 ->
-    Γ ⊢t e ⋮t T2 ->
-    T1 = T2.
+Class BasicTypingUnique (E: Type) `{Typing tyctx E ty} := basic_typing_unique: forall (Γ: tyctx) (e: E) (T1 T2: ty), Γ ⊢ e ⋮ T1 -> Γ ⊢ e ⋮ T2 -> T1 = T2.
+
+#[global] Instance BasicTypingUnique_tm: BasicTypingUnique tm.
 Proof.
+  unfold BasicTypingUnique.
   intros * H. revert T2. revert_all.
   apply (tm_has_type_mutual_rec
-           (fun Γ v T1 _ => ∀ T2, Γ ⊢t v ⋮v T2 → T1 = T2)
-           (fun Γ e T1 _ => ∀ T2, Γ ⊢t e ⋮t T2 → T1 = T2));
+           (fun Γ v T1 _ => ∀ T2, Γ ⊢ v ⋮ T2 → T1 = T2)
+           (fun Γ e T1 _ => ∀ T2, Γ ⊢ e ⋮ T2 → T1 = T2));
     intros;
     try match goal with
-      | H : _ ⊢t _ ⋮t _ |- _ => sinvert H
-      | H : _ ⊢t _ ⋮v _ |- _ => sinvert H
-      end; eauto;
+      | H : _ ⊢ _ ⋮ _ |- _ => sinvert H
+      end; simplify_map_eq; eauto; fold_typing_class;
     try solve [ auto_pose_fv x; repeat specialize_with x; hauto ].
-  by simplify_map_eq.
 Qed.
+Arguments BasicTypingUnique_tm /.
 
-Lemma basic_typing_value_unique: forall Γ v T1 T2,
-    Γ ⊢t v ⋮v T1 ->
-    Γ ⊢t v ⋮v T2 ->
-    T1 = T2.
+#[global] Instance BasicTypingUnique_value: BasicTypingUnique value.
 Proof.
+  unfold BasicTypingUnique.
   intros * H. revert T2. revert_all.
   apply (value_has_type_mutual_rec
-           (fun Γ v T1 _ => ∀ T2, Γ ⊢t v ⋮v T2 → T1 = T2)
-           (fun Γ e T1 _ => ∀ T2, Γ ⊢t e ⋮t T2 → T1 = T2));
+           (fun Γ v T1 _ => ∀ T2, Γ ⊢ v ⋮ T2 → T1 = T2)
+           (fun Γ e T1 _ => ∀ T2, Γ ⊢ e ⋮ T2 → T1 = T2));
     intros;
     try match goal with
-      | H : _ ⊢t _ ⋮t _ |- _ => sinvert H
-      | H : _ ⊢t _ ⋮v _ |- _ => sinvert H
-      end; eauto;
+      | H : _ ⊢ _ ⋮ _ |- _ => sinvert H
+      | H : _ ⊢ _ ⋮ _ |- _ => sinvert H
+      end; simplify_map_eq; eauto; fold_typing_class;
     try solve [ auto_pose_fv x; repeat specialize_with x; hauto ].
-  by simplify_map_eq.
 Qed.
-
+Arguments BasicTypingUnique_value /.
 (** * Strengthening lemmas *)
+
+Ltac aset_solver :=
+try match goal with
+  | [H: <[?x:=_]> ?Γ !! ?y = _ |- ?Γ !! ?y = _ ] =>
+        solve [rewrite lookup_insert_ne in * by fast_set_solver!!; eauto]
+end;
+repeat match goal with
+| [H:  <[?x:=_]> _ !! ?x = _ |- _ ] =>
+  setoid_rewrite lookup_insert in H; eauto; simplify_eq
+| [H: <[?y:=_]> _ !! ?x = _ |- _ ] =>
+  assert (x ≠ y) by fast_set_solver!!;
+  setoid_rewrite lookup_insert_ne in H; eauto; simplify_eq
+| [|- <[?x:=_]> _ !! ?x = _ ] =>
+  setoid_rewrite lookup_insert; eauto
+| [|- <[?y:=_]> _ !! ?x = _ ] =>
+  assert (x ≠ y) by fast_set_solver!!;
+  setoid_rewrite lookup_insert_ne; eauto
+| [ |- ∅ ⊆ ?M ] =>
+  match type of M with
+  | amap _ => apply map_empty_subseteq
+  end
+end.
+
+Ltac lc_set_solver :=
+  lc_solver;
+  match goal with
+  | [ |- ?x # {_ ~> _} _] =>
+        solve [eapply not_elem_of_weaken; [ | apply open_fv ]; ln_simpl; fast_set_solver!!]
+  | [ |- _ !! _ = _ ] => aset_solver
+  | [ |- _ ⊆ ?M ] =>
+    match type of M with
+    | amap _ => aset_solver
+    | _ => fast_set_solver!!
+    end
+  | _ => fast_set_solver!!
+  end. 
 
 (* This statement can be generalized to taking a union of the context and a
 disjoint new context. *)
 Lemma basic_typing_strengthen_tm: forall Γ x Tx (v: tm) T,
-    (<[x:=Tx]>Γ) ⊢t v ⋮t T -> x # v -> Γ ⊢t v ⋮t T
+    (<[x:=Tx]>Γ) ⊢ v ⋮ T -> x # v -> Γ ⊢ v ⋮ T
 with basic_typing_strengthen_value: forall Γ x Tx (v: value) T,
-    (<[x:=Tx]>Γ) ⊢t v ⋮v T -> x # v -> Γ ⊢t v ⋮v T.
+    (<[x:=Tx]>Γ) ⊢ v ⋮ T -> x # v -> Γ ⊢ v ⋮ T.
 Proof.
   all : intros * H Hfresh; remember (<[x:=Tx]>Γ);
     generalize dependent Γ;
-    destruct H; intros; unfold context in *; subst;
-    econstructor; eauto;
-    try solve [
-        try instantiate_atom_listctx;
-        try rewrite insert_commute in * by my_set_solver;
-        auto_eapply; eauto;
-        match goal with
-        | |- context [{_ ~t> _} _] =>
-            eapply not_elem_of_weaken; [ | apply open_fv_tm ]; my_set_solver
-        | _ => my_set_solver
-        end ].
-  by rewrite lookup_insert_ne in * by my_set_solver.
+    destruct H; intros; unfold tyctx in *; subst.
+    econstructor_L; ln_simpl; fold_typing_class.
+    all:
+      econstructor_L; auto_specialization; ln_simpl; fold_typing_class;
+      try rewrite insert_commute in * by my_set_solver;
+      match goal with
+      | [ |-  _ !! _ = _ ] => lc_set_solver
+      | H: <[ ?x := ?Tx]> ?Γ ⊢ ?e ⋮ _ |- ?Γ ⊢ ?e ⋮ _ => 
+        auto_eapply; eauto; lc_set_solver
+      end.
 Qed.
+
+Class BasicTypingStrengthen (E: Type) `{Typing tyctx E ty} `{Stale E} := basic_typing_strengthen: forall (Γ: tyctx) (x: atom) (Tx: ty) (e: E) (T: ty), (<[x:=Tx]>Γ) ⊢ e ⋮ T -> x # e -> Γ ⊢ e ⋮ T.
+
+#[global] Instance BasicTypingStrengthen_tm: BasicTypingStrengthen tm.
+Proof.
+  unfold BasicTypingStrengthen.
+  eapply basic_typing_strengthen_tm; eauto.
+Qed.
+Arguments BasicTypingStrengthen_tm /.
+
+#[global] Instance BasicTypingStrengthen_value: BasicTypingStrengthen value.
+Proof.
+  unfold BasicTypingStrengthen.
+  eapply basic_typing_strengthen_value; eauto.
+Qed.
+Arguments BasicTypingStrengthen_value /.
 
 (** * Type properties of syntax sugar *)
 
+Ltac auto_specialization :=
+  try lazymatch goal with
+  | |- forall y, y ∉ _ -> _ =>
+    let y := fresh "y" in
+    let Hy := fresh "Hy" in
+    intros y Hy;
+    repeat specialize_with y
+  end;
+  eauto.
+
+Ltac L_econstructor_specialized :=
+  econstructor_L; auto_specialization; ln_simpl.
+
+Ltac basic_typing_solver :=
+fold_typing_class;
+repeat
+ (match goal with
+| [H: ?g ⊢ (treturn ?v) ⋮ ?t |- ?g ⊢ ?v ⋮ ?t ] => sinvert H; eauto
+| [ H: ?g ⊢ ?e ⋮ ?T, H': ?g ⊢ ?e ⋮ ?T |- _ ] => clear H'
+| [ H: ?g ⊢ ?e ⋮ ?T, H': ?g ⊢ ?e ⋮ ?T |- _ ] => clear H'
+| [ H: ?g ⊢ ?e ⋮ ?T, H': ?g ⊢ ?e ⋮ ?T' |- _ ] =>
+     assert (T = T') by eauto using basic_typing_unique; subst
+| [H: ∅ ⊢ ?e ⋮ _ |- _ ⊢ ?e ⋮ _ ] =>
+  eapply basic_typing_weaken in H; eauto; try lc_set_solver
+| [H: ?Γ ⊢ ?e ⋮ _ |- <[ _ := _ ]> ?Γ ⊢ ?e ⋮ _ ] =>
+  apply basic_typing_weaken_insert; eauto; lc_set_solver
+| [H: <[ _ := _ ]> ?Γ ⊢ ?e ⋮ _ |-  ?Γ ⊢ ?e ⋮ _ ] =>
+  apply basic_typing_strengthen in H; eauto; lc_set_solver
+| [H: _ ⊢ ?e ^^ (vfvar ?z) ⋮ _ |- _ ⊢ ?e ^^ _ ⋮ _ ] =>
+  eapply basic_typing_open in H; eauto; try lc_set_solver
+| |- _ ⊢ (vfvar ?x) ⋮ _ =>
+  econstructor; aset_solver
+| |- _ ⊢ _ ⋮ _ =>
+  L_econstructor_specialized; smart_ln_simpl
+end; fold_typing_class; eauto).
+
 Lemma mk_app_has_type Γ e v T1 T2 :
-  Γ ⊢t e ⋮t T1 ⤍ T2 ->
-  Γ ⊢t v ⋮t T1 ->
-  Γ ⊢t mk_app e v ⋮t T2.
+  Γ ⊢ e ⋮ T1 ⤍ T2 ->
+  Γ ⊢ v ⋮ T1 ->
+  Γ ⊢ mk_app e v ⋮ T2.
 Proof.
   intros.
-  econstructor; eauto.
   assert (lc e) by basic_typing_regular_simp.
   assert (lc v) by basic_typing_regular_simp.
-  instantiate_atom_listctx.
-  simpl. rewrite open_rec_lc_tm; eauto.
-  econstructor. apply basic_typing_weaken_insert_tm; eauto. my_set_solver.
-  auto_exists_L_intros.
-  econstructor. instantiate (1 := T2). instantiate (1 := T1).
-  econstructor. setoid_rewrite lookup_insert_ne. setoid_rewrite lookup_insert. eauto. my_set_solver.
-  econstructor. simplify_map_eq; eauto.
-  auto_exists_L_intros.
-  econstructor. econstructor. simplify_map_eq; eauto.
+  basic_typing_solver.
 Qed.
 
+Ltac basic_typing_destruct :=
+fold_typing_class;
+repeat (match goal with
+| [H: _ ⊢ tlete _ _ ⋮ ?T2 |- _ ] =>
+  sinvert H; ln_simpl;
+  let x := fresh "x" in
+  auto_pose_fv x; repeat specialize_with x; smart_ln_simpl
+| [H: _ ⊢ tletapp _ _ _ ⋮ ?T2 |- _ ] =>
+  sinvert H; ln_simpl;
+  let x := fresh "x" in
+  auto_pose_fv x; repeat specialize_with x; smart_ln_simpl
+| [H: _ ⊢ (vfvar ?x) ⋮ _ |- _ ] =>
+  sinvert H; ln_simpl; aset_solver
+| [H: _ ⊢ (treturn _) ⋮ _ |- _ ] =>
+  sinvert H; ln_simpl
+end; fold_typing_class; eauto).
+
 Lemma mk_app_has_type_inv Γ e v T2 :
-  Γ ⊢t mk_app e v ⋮t T2 ->
+  Γ ⊢ mk_app e v ⋮ T2 ->
   lc v ->
-  exists T1, Γ ⊢t e ⋮t T1 ⤍ T2 /\ Γ ⊢t v ⋮t T1.
+  exists T1, Γ ⊢ e ⋮ T1 ⤍ T2 /\ Γ ⊢ v ⋮ T1.
 Proof.
-  intros.
-  sinvert H. simpl in H6. auto_pose_fv x. repeat specialize_with x.
-  rewrite open_rec_lc_tm in H6 by auto.
-  sinvert H6. remember x. auto_pose_fv y. repeat specialize_with y.
-  sinvert H8. simpl in H12. auto_pose_fv z. repeat specialize_with z. subst.
-  sinvert H12. sinvert H7. setoid_rewrite lookup_insert in H8. simplify_eq.
-  sinvert H11. setoid_rewrite lookup_insert in H7. simplify_eq.
-  sinvert H9. setoid_rewrite lookup_insert_ne in H7. setoid_rewrite lookup_insert in H7. simplify_eq.
-  exists T3. intuition; eauto.
-  eapply basic_typing_strengthen_tm; eauto.
-  all: my_set_solver.
+  unfold mk_app. intros.
+  basic_typing_destruct.
+  eexists; split; eauto. basic_typing_solver.
 Qed.
 
 (** * Type preservation *)
@@ -297,32 +493,45 @@ Proof.
   induction 1; eauto.
 Qed.
 
+Lemma eval_op_typing (op: effop) (c1 c: constant) :
+  ⇓{op~c1}{c} ->
+  exists T1 T2, ty_of_op op = T1 ⤍ T2 /\
+  ∅ ⊢ (vconst c1) ⋮ T1 /\ ∅ ⊢ (vconst c) ⋮ T2.
+Proof.
+  intros * H. invclear H.
+  - eexists TNat, TNat. repeat split; eauto; econstructor.
+  - eexists TNat, TBool. repeat split; eauto; econstructor.
+  - eexists TNat, TNat. repeat split; eauto; econstructor.
+Qed.
+
 (** perservation *)
-Lemma preservation: forall Γ T (e e': tm), e ↪ e' -> Γ ⊢t e ⋮t T -> Γ ⊢t e' ⋮t T.
+Lemma preservation: forall Γ T (e e': tm), e ↪ e' -> Γ ⊢ e ⋮ T -> Γ ⊢ e' ⋮ T.
 Proof.
   intros * Hstep HT. move HT at top. revert_all.
-  induction 1; intros; sinvert Hstep; eauto.
-  - auto_pose_fv x. repeat specialize_with x.
-    rewrite <- subst_intro_tm with (x:=x) by (eauto; my_set_solver).
-    sinvert HT. eauto using basic_typing_subst_tm.
-  - auto_pose_fv x. repeat specialize_with x.
-    rewrite <- subst_intro_tm with (x:=x) by (eauto; my_set_solver).
-    sinvert H0. erewrite <- tr_reduction_sound in H1; eauto.
-    eauto using basic_typing_subst_tm.
-  - sinvert H.
-    econstructor; eauto.
-    auto_pose_fv x. repeat specialize_with x.
-    rewrite <- subst_intro_tm with (x:=x) by (eauto; my_set_solver).
-    eauto using basic_typing_subst_tm.
-  - sinvert H.
-    econstructor; eauto.
-    auto_pose_fv x. repeat specialize_with x.
-    rewrite <- subst_intro_value with (x:=x) by (eauto; my_set_solver).
-    eauto using basic_typing_subst_value.
+  induction 1; intros; sinvert Hstep;
+  (* auto_pose_fv x; repeat specialize_with x; *)
+  eauto; basic_typing_solver.
+  - basic_typing_destruct; 
+    auto_pose_fv x; repeat specialize_with x;
+    basic_typing_solver.
+  - auto_pose_fv x; repeat specialize_with x.
+    basic_typing_solver.
+    apply eval_op_typing in H10; simp_hyps. 
+    rewrite H4 in H0. simp_hyps.
+    unfold tyctx in *;
+    basic_typing_solver.
+  - sinvert H; ln_simpl.
+    auto_pose_fv x; repeat specialize_with x.
+    basic_typing_solver.
+  - sinvert H; ln_simpl.
+    auto_pose_fv x; repeat specialize_with x.
+    (* ln_simpl has evaluated the terms too much **)
+    rewrite open_vlam_rev in *;
+    basic_typing_solver.
 Qed.
 
 (** multi preservation *)
-Lemma multi_preservation: forall Γ T (e e': tm),e ↪* e' -> Γ ⊢t e ⋮t T -> Γ ⊢t e' ⋮t T.
+Lemma multi_preservation: forall Γ T (e e': tm),e ↪* e' -> Γ ⊢ e ⋮ T -> Γ ⊢ e' ⋮ T.
 Proof.
   induction 1; eauto using preservation.
 Qed.
@@ -332,18 +541,3 @@ Ltac pure_multistep_tac :=
   | [H: _ |- (treturn ?v) ↪* (treturn _) ] =>
       apply (value_reduction_any_ctx v); eauto
   end; basic_typing_regular_simp.
-
-Ltac unique_basic_type :=
-  repeat match goal with
-    | [ H: ?g ⊢t ?e ⋮t ?T, H': ?g ⊢t ?e ⋮t ?T |- _ ] => clear H'
-    | [ H: ?g ⊢t ?e ⋮v ?T, H': ?g ⊢t ?e ⋮v ?T |- _ ] => clear H'
-    | [ H: ?g ⊢t ?e ⋮t ?T, H': ?g ⊢t ?e ⋮t ?T' |- _ ] =>
-        assert (T = T') by eauto using basic_typing_tm_unique; subst
-    | [ H: ?g ⊢t ?e ⋮v ?T, H': ?g ⊢t ?e ⋮v ?T' |- _ ] =>
-        assert (T = T') by eauto using basic_typing_value_unique; subst
-    end.
-
-Ltac basic_typing_solver :=
-  match goal with
-  | [H: ?g ⊢t (treturn ?v) ⋮t ?t |- ?g ⊢t ?v ⋮v ?t ] => sinvert H; eauto
-  end.
