Instantiation.v
@@ -1,55 +1,73 @@
 From stdpp Require Import mapset.
-From CT Require Import CoreLang.
-From CT Require Import CoreLangProp.
+From CT Require Import Syntax.
 From CT Require Import OperationalSemantics.
 From CT Require Import BasicTypingProp.
-From CT Require Import Qualifier.
-From CT Require Import RefinementType.
 
-Import Atom.
-Import CoreLang.
-Import Tactics.
-Import NamelessTactics.
-Import OperationalSemantics.
-Import BasicTyping.
-Import RefinementType.
+Import BaseDef MyTactics Primitives Lang LangLc Qualifier OperationalSemantics BasicTyping BasicTypingProp.
 
 (** This file defines valuation environment, i.e., substitution (σ), and
   multi-substitution operation. *)
 
 (** Environment (substitution) *)
 Notation env := (amap value).
+(** A world is a set of substitutions that satisfies a proposition.
+    π ⊧ P iff ∀ σ ∈ π, σ ⊧ P.
+    If π ⊧ P and P -> Q, then π ⊧ Q.
+    A world can also be treated as an abstraction of a set of propositions P (closed under implication).
+    The denotation of a type context is the set of propositions that are satisfied under the type context—a set of worlds (not a single world, because it may not be closed under implication).
+    ⟦Γ⟧ := { π | Γ ⊧ P ∧ π ⊧ P }
+    Γ ⊧ P iff there exists a world π in ⟦Γ⟧.
+    Assume mkWorld(P) is the minimal set of substitutions that satisfies P.
+    mkWorld(P) := {σ ∈ E | σ ⊧ P}
+    ⟦Γ⟧ := { mkWorld(P) | Γ ⊧ P }, closed with respect to the subset relation.
+    For example, mkWorld(x = y) :=
+      {[x := True, y := True], [x := False, y := False]}
+    For a world π = {[x := True, y := True]}, π ⊧ x = y.
+    For a type context x:{bool | v = True}, y:{bool | top },
+    its denotation contains all worlds including 
+    [x := True, y := True] and [x := True, y := False].
+    ⟦Γ⟧ = {
+      {[x := True, y := True], [x := True, y := False]}, 
+      {[x := True, y := True], [x := True, y := False], [x := False, y := False]},
+      ..., 
+    }
+    This means that it is free to pick any world from the denotation; if the world can entail the proposition P, it is sufficient to prove the proposition P.
+    For a type context x:{bool | v = True}, y:[bool | top ],
+    its denotation contains all worlds including 
+    [x := True, y := True] or [x := True, y := False].
+    ⟦Γ⟧ = {
+      {[x := True, y := True]}, 
+      {[x := True, y := False]},
+      {[x := True, y := False], [x := False, y := False]},
+      ..., 
+    }
+    For a type context x:[bool | top], y:[bool | v = x ],
+    its denotation contains all worlds including 
+    [x := True, y := True] or [x := False, y := False].
+    For a type context x:{bool | top}, y:[bool | v = x ],
+    its denotation contains all worlds including 
+    [x := True, y := True] and [x := False, y := False].
+*)
+Inductive world : Type :=
+| World (L: aset) (π: env -> Prop).
+(* Technically, we require the domain of all substitutions in the world to be the same (i.e., L). *)
 
-Inductive epr : Type :=
-| Epr (σ: env) (L: aset) (Σ: env -> Prop).
+Definition closed_env (env : env) := map_Forall (fun _ v => stale v ≡ ∅) env.
 
-Definition closed_env (env : env) := map_Forall (fun _ => closed_value) env.
-Inductive closed_epr: epr -> Prop :=
-| Closed_epr: forall (σ: env) (L: aset) (Σ: env -> Prop),
-    dom σ ∩ L = ∅ ->
-    closed_env σ ->
-    (forall σ', Σ σ' -> closed_env σ /\ dom σ' = L) ->
-    closed_epr (Epr σ L Σ).
+Inductive closed_world: world -> Prop :=
+| ClosedWorld: forall L π,
+    forall σ, π σ -> dom σ ≡ L /\ closed_env σ ->
+    closed_world (World L π).
 
-Definition eprdom (epr: epr) :=
-  match epr with
-  | Epr σ L _ => dom σ ∪ L
+#[global] Instance world_stale {A:Type} : Stale world := 
+  fun w => match w with
+  | World L π => L
   end.
-
-Inductive eprR: epr -> env -> Prop :=
-| EprR: forall σ1 σ2 L Σ, Σ σ2 -> eprR (Epr σ1 L Σ) (σ1 ∪ σ2).
-
-#[global]
-  Instance epr_stale {A:Type} : Stale epr := eprdom.
-Arguments epr_stale /.
+Arguments world_stale /.
 
 (** Multi-substitution, i.e., σ(⋅) operation. The definition is parameterized by
   any substitution. *)
-Definition msubst {A} (subst : atom -> value -> A -> A)
-                  (env : env) (a : A) : A :=
+Definition msubst {A: Type} (a : A) `{Subst value A}  (env : env)  : A :=
   map_fold subst a env.
 
-Notation "'m{' x '}q'" := (msubst qualifier_subst x) (at level 20, format "m{ x }q", x constr).
-Notation "'m{' x '}r'" := (msubst rty_subst x) (at level 20, format "m{ x }r", x constr).
-Notation "'m{' x '}v'" := (msubst value_subst x) (at level 20, format "m{ x }v", x constr).
-Notation "'m{' x '}t'" := (msubst tm_subst x) (at level 20, format "m{ x }t", x constr).
+Notation "'m{' x '}'" := (msubst x) (at level 20, format "m{ x }", x constr).
