LocallyNameless/FineRty.v
@@ -1,25 +1,19 @@
 Require Import Stdlib.Program.Wf.
 From stdpp Require Import mapset.
 From stdpp Require Import natmap.
-From CT Require Import Syntax.
+From CT Require Import BaseDef MyTactics ListCtx.
+From CT.Syntax Require Import Lang Primitives Qualifier RefinementType Syntax.
 
-Import BaseDef.
-Import Lang.
-Import MyTactics.
-Import Primitives.
-Import Qualifier.
-Import ListCtx.
-Import List.
-Import Syntax.
+Import BaseDef Lang MyTactics Primitives Qualifier ListCtx List RefinementType Syntax.
 
 Lemma ok_ctx_ok: forall Γ, ok_ctx Γ -> ok Γ.
 Proof.
   induction 1; eauto.
 Qed.
 
-Class OpenPreserve {A: Type} (predA: A -> Prop) `{Open value A} := open_preserve: forall (e: A) (k: nat) (v: value), predA e <-> predA ({k ~> v} e).
+Class OpenPreserve {A: Type} (predA: A -> Prop) `{Open value A} := open_preserve: forall (e: A) (k: nat) (v: value), predA ({k ~> v} e) <-> predA e.
 
-Class SubstPreserve {A: Type} (predA: A -> Prop) `{Subst value A} := subst_preserve: forall (e: A) (x: atom) (v: value), predA e <-> predA ({x := v} e).
+Class SubstPreserve {A: Type} (predA: A -> Prop) `{Subst value A} := subst_preserve: forall (e: A) (x: atom) (v: value), predA ({x := v} e) <-> predA e.
 
 #[global] Instance OpenPreserve_is_over_base_rty: OpenPreserve is_over_base_rty.
 Proof.
@@ -71,35 +65,6 @@ Qed.
 
 Lemma is_coverage_open_rty_aux n: forall τ, rty_measure τ <= n -> forall k (v_x: value), is_coverage_rty ({ k ~> v_x} τ) <-> is_coverage_rty τ.
 Proof.
-  induction n; split; intros HH; invclear HH; simplify_eq; eauto; ln_simpl;
-  try solve [pose (rty_measure_gt_0 τ); lia].
-  - simpl. destruct τ; sinvert H.
-  - destruct τ; sinvert H.
-  - destruct τ.
-    + sinvert HH; eauto.
-    + sinvert HH; eauto.
-    + destruct τ1; sinvert HH; eauto; econstructor; rewrite <- IHn; eauto; simpl in *; lia.
-  - destruct τ.
-    + sinvert HH; eauto.
-    + simpl. eauto.
-    + destruct τ1; sinvert HH; eauto; simpl; econstructor; try solve [rewrite IHn; eauto; simpl in *; lia].
-      * rewrite <- IHn in H2; eauto; simpl in *; lia.
-Qed.
-
-#[global] Instance OpenPreserve_is_coverage_rty: OpenPreserve is_coverage_rty.
-Proof.
-  unfold OpenPreserve. intros e.
-  remember (rty_measure e) as n. generalize dependent e.
-  induction n; split; intros H; invclear H; simplify_eq; eauto; simpl in *;
-  try solve [pose (rty_measure_gt_0 e); lia].
-  - rewrite <- IHn; eauto. simplify_eq. simpl.  
-  -  
-  split; induction e; simpl; intros; inversion H; subst; eauto; try hauto.
-Qed.
-Arguments OpenPreserve_is_coverage_rty /.
-
-Lemma is_coverage_open_rty_aux n: forall τ, rty_measure τ <= n -> forall k (v_x: value), is_coverage_rty ({ k ~> v_x} τ) <-> is_coverage_rty τ.
-Proof.
   induction n; split; intros HH.
   - destruct τ; sinvert H.
   - destruct τ; sinvert H.
@@ -109,13 +74,17 @@ Proof.
     + destruct τ1; sinvert HH; eauto; econstructor; rewrite <- IHn; eauto; simpl in *; lia.
   - destruct τ.
     + sinvert HH; eauto.
-    + simpl. eauto.
-    + destruct τ1; sinvert HH; eauto; simpl; econstructor; try solve [rewrite IHn; eauto; simpl in *; lia].
+    + ln_simpl. eauto.
+    + destruct τ1; sinvert HH; eauto; simpl; econstructor; try solve [rewrite IHn; eauto; ln_simpl; lia].
       * rewrite <- IHn in H2; eauto; simpl in *; lia.
 Qed.
 
-Lemma is_coverage_open_rty: forall τ, forall k (v_x: value), is_coverage_rty ({ k ~> v_x} τ) <-> is_coverage_rty τ.
-Proof. eauto using is_coverage_open_rty_aux. Qed.
+#[global] Instance OpenPreserve_is_coverage_rty: OpenPreserve is_coverage_rty.
+Proof.
+  unfold OpenPreserve. intros.
+  rewrite is_coverage_open_rty_aux; eauto.
+Qed.
+Arguments OpenPreserve_is_coverage_rty /.
 
 Lemma is_coverage_rty_subst_aux n: forall τ, rty_measure τ <= n -> forall x (v_x: value), is_coverage_rty ({ x := v_x} τ) <-> is_coverage_rty τ.
 Proof.
@@ -128,13 +97,17 @@ Proof.
     + destruct τ1; sinvert HH; eauto; econstructor; rewrite <- IHn; eauto; simpl in *; lia.
   - destruct τ.
     + sinvert HH; eauto.
-    + simpl. eauto.
+    + ln_simpl. eauto.
     + destruct τ1; sinvert HH; eauto; simpl; econstructor; try solve [rewrite IHn; eauto; simpl in *; lia].
       * rewrite <- IHn in H2; eauto; simpl in *; lia.
 Qed.
 
-Lemma is_coverage_rty_subst: forall τ x (v_x: value), is_coverage_rty ({ x := v_x} τ) <-> is_coverage_rty τ.
-Proof. eauto using is_coverage_rty_subst_aux. Qed.
+#[global] Instance SubstPreserve_is_coverage_rty: SubstPreserve is_coverage_rty.
+Proof.
+  unfold SubstPreserve. intros.
+  rewrite is_coverage_rty_subst_aux; eauto.
+Qed.
+Arguments SubstPreserve_is_coverage_rty /.
 
 Lemma open_rty_arr_rev: forall ρ τ k v, (({k ~> v} ρ) ⇨ ({S k ~> v} τ)) = {k ~> v} (ρ ⇨ τ).
 Proof. eauto. Qed.
@@ -152,28 +125,28 @@ Ltac fine_rty_aux_simp_aux :=
       setoid_rewrite open_rty_arr_rev
   | [H: _ |- context [ (({?x := ?v} _) ⇨ ({?x := ?v} _)) ] ] =>
       setoid_rewrite rty_subst_arr_rev
-  | [H: context [ is_over_base_rty ({_ ~> _} ?τ) ] |- _ ] => setoid_rewrite is_over_base_open_rty in H
-  | [H: context [ is_over_base_rty ({_ := _} ?τ) ] |- _ ] => setoid_rewrite is_over_base_rty_subst in H
-  | [H: _ |- context [ is_over_base_rty ({_ ~> _} ?τ) ] ] => setoid_rewrite is_over_base_open_rty
-  | [H: _ |- context [ is_over_base_rty ({_ := _} ?τ) ] ] => setoid_rewrite is_over_base_rty_subst
-  | [H: context [ is_under_base_rty ({_ ~> _} ?τ) ] |- _ ] => setoid_rewrite is_under_base_open_rty in H
-  | [H: context [ is_under_base_rty ({_ := _} ?τ) ] |- _ ] => setoid_rewrite is_under_base_rty_subst in H
-  | [H: _ |- context [ is_under_base_rty ({_ ~> _} ?τ) ] ] => setoid_rewrite is_under_base_open_rty
-  | [H: _ |- context [ is_under_base_rty ({_ := _} ?τ) ] ] => setoid_rewrite is_under_base_rty_subst
-  | [H: context [ is_coverage_rty ({_ ~> _} ?τ) ] |- _ ] => setoid_rewrite is_coverage_open_rty in H
-  | [H: context [ is_coverage_rty ({_ := _} ?τ) ] |- _ ] => setoid_rewrite is_coverage_rty_subst in H
-  | [H: _ |- context [ is_coverage_rty ({_ ~> _} ?τ) ] ] => setoid_rewrite is_coverage_open_rty
-  | [H: _ |- context [ is_coverage_rty ({_ := _} ?τ) ] ] => setoid_rewrite is_coverage_rty_subst
+  | [H: context [ is_over_base_rty ({_ ~> _} ?τ) ] |- _ ] => setoid_rewrite open_preserve in H
+  | [H: context [ is_over_base_rty ({_ := _} ?τ) ] |- _ ] => setoid_rewrite subst_preserve in H
+  | [H: context [ is_under_base_rty ({_ ~> _} ?τ) ] |- _ ] => setoid_rewrite open_preserve in H
+  | [H: context [ is_under_base_rty ({_ := _} ?τ) ] |- _ ] => setoid_rewrite subst_preserve in H
+  | [H: context [ is_coverage_rty ({_ ~> _} ?τ) ] |- _ ] => setoid_rewrite open_preserve in H
+  | [H: context [ is_coverage_rty ({_ := _} ?τ) ] |- _ ] => setoid_rewrite subst_preserve in H
+  | [H: _ |- context [ is_under_base_rty ({_ ~> _} ?τ) ] ] => setoid_rewrite open_preserve
+  | [H: _ |- context [ is_under_base_rty ({_ := _} ?τ) ] ] => setoid_rewrite subst_preserve
+  | [H: _ |- context [ is_over_base_rty ({_ ~> _} ?τ) ] ] => setoid_rewrite open_preserve
+  | [H: _ |- context [ is_over_base_rty ({_ := _} ?τ) ] ] => setoid_rewrite subst_preserve
+  | [H: _ |- context [ is_coverage_rty ({_ ~> _} ?τ) ] ] => setoid_rewrite open_preserve
+  | [H: _ |- context [ is_coverage_rty ({_ := _} ?τ) ] ] => setoid_rewrite subst_preserve
   end.
 
 Lemma fine_open_rty τ: forall k (v_x: value), fine_rty ({ k ~> v_x} τ) <-> fine_rty τ.
 Proof.
-  split; intros; destruct τ; simpl in *; repeat fine_rty_aux_simp_aux; eauto.
+  split; intros; destruct τ; simpl in *; eauto; fine_rty_aux_simp_aux; eauto.
 Qed.
 
 Lemma fine_rty_subst: forall τ x (v_x: value), fine_rty ({ x := v_x} τ) <-> fine_rty τ.
 Proof.
-  split; intros; destruct τ; simpl in *; repeat fine_rty_aux_simp_aux; eauto.
+    split; intros; destruct τ; simpl in *; eauto; fine_rty_aux_simp_aux; eauto.
 Qed.
 
 Ltac fine_rty_simp_aux :=
@@ -186,26 +159,26 @@ Ltac fine_rty_simp_aux :=
       setoid_rewrite open_rty_arr_rev
   | [H: _ |- context [ (({?x := ?v} _) ⇨ ({?x := ?v} _)) ] ] =>
       setoid_rewrite rty_subst_arr_rev
-  | [H: context [ fine_rty ({_ ~> _} ?τ) ] |- _ ] => setoid_rewrite fine_open_rty in H
-  | [H: context [ fine_rty ({_ := _} ?τ) ] |- _ ] => setoid_rewrite fine_rty_subst in H
-  | [H: _ |- context [ fine_rty ({_ ~> _} ?τ) ] ] => setoid_rewrite fine_open_rty
-  | [H: _ |- context [ fine_rty ({_ := _} ?τ) ] ] => setoid_rewrite fine_rty_subst
+  | [H: context [ fine_rty ({_ ~> _} ?τ) ] |- _ ] => setoid_rewrite open_preserve in H
+  | [H: context [ fine_rty ({_ := _} ?τ) ] |- _ ] => setoid_rewrite subst_preserve in H
+  | [H: _ |- context [ fine_rty ({_ ~> _} ?τ) ] ] => setoid_rewrite open_preserve
+  | [H: _ |- context [ fine_rty ({_ := _} ?τ) ] ] => setoid_rewrite subst_preserve
   | _ => fine_rty_aux_simp_aux
   end.
 
-Lemma lc_rty_under_base_q: forall b ϕ, lc_rty ([:b|ϕ]) <-> lc_phi1 ϕ.
+Lemma lc_under_base_q: forall b ϕ, lc ([:b|ϕ]) <-> body ϕ.
 Proof.
   split; intros; sinvert H; eauto.
   econstructor; eauto. exists x. eauto. simpl; eauto.
 Qed.
 
-Lemma lc_rty_over_base_q: forall b ϕ, lc_rty ({:b|ϕ}) <-> lc_phi1 ϕ.
+Lemma lc_over_base_q: forall b ϕ, lc ({:b|ϕ}) <-> body ϕ.
 Proof.
   split; intros; sinvert H; eauto.
   econstructor; eauto. exists x. eauto. simpl; eauto.
 Qed.
 
-Lemma lc_rty_base_flip: forall b ϕ, lc_rty {:b|ϕ} <-> lc_rty [:b|ϕ].
+Lemma lc_base_flip: forall b ϕ, lc {:b|ϕ} <-> lc [:b|ϕ].
 Proof.
   split; intros; sinvert H; econstructor; eauto.
 Qed.
@@ -213,19 +186,19 @@ Qed.
 Lemma closed_rty_base_flip: forall L b ϕ, closed_rty L {:b|ϕ} <-> closed_rty L [:b|ϕ].
 Proof.
   split; intros; sinvert H; econstructor; eauto;
-  rewrite lc_rty_base_flip in *; eauto.
+  rewrite lc_base_flip in *; eauto.
 Qed.
 
-Lemma lc_rty_arr: forall ρ τ, lc_rty (ρ ⇨ τ) <-> fine_rty (ρ ⇨ τ) /\ lc_rty ρ /\ body_rty τ.
+Lemma lc_rty_arr: forall ρ τ, lc (ρ ⇨ τ) <-> fine_rty (ρ ⇨ τ) /\ lc ρ /\ body τ.
 Proof.
   split; intros; sinvert H.
   - intuition. auto_exists_L.
-  - unfold body_rty in H1. simp_hyps. auto_exists_L; eauto.
+  - unfold body in H1. simp_hyps. auto_exists_L; eauto.
 Qed.
 
 Lemma closed_rty_arr:
   ∀ (L : aset) (ρ τ : rty),
-    closed_rty L (ρ⇨τ) ↔ (fine_rty (ρ⇨τ)) /\ closed_rty L ρ ∧ body_rty τ /\ (rty_fv τ ⊆ L).
+    closed_rty L (ρ⇨τ) ↔ (fine_rty (ρ⇨τ)) /\ closed_rty L ρ ∧ body τ /\ (stale τ ⊆ L).
 Proof.
   split; intros.
   - sinvert H. rewrite lc_rty_arr in H0. intuition.
@@ -241,9 +214,10 @@ Ltac fine_rty_simp := simpl in *; repeat fine_rty_simp_aux.
 Ltac fine_rty_solver := fine_rty_simp; eauto.
 
 Ltac solve_fine_rty :=
+  fold_syntax_class;
   repeat fine_rty_simp_aux; eauto;
   match goal with
-  | [ _ : _ |- context [rty_subst _ _ ?ρ] ] =>
+  | [ _ : _ |- context [subst _ _ ?ρ] ] =>
       destruct ρ; simpl in *; eauto; intuition
   | [ _ : _ |- fine_rty _ ] =>
       simpl in *;
