OperationalSemantics.v
@@ -1,11 +1,9 @@
 From stdpp Require Import mapset.
-From CT Require Import CoreLang.
-From CT Require Import CoreLangProp.
+From CT.Syntax Require Import Syntax.
+From CT.LocallyNameless Require Import Lc.
 
-Import Atom.
-Import CoreLang.
-Import Tactics.
-Import NamelessTactics.
+Import BaseDef MyTactics Primitives Lang Lc.
+Import LangLc.
 
 Inductive eval_op: effop -> constant -> constant -> Prop :=
 | eval_op_plus_one: forall (a: nat), eval_op op_plus_one a (1 + a)
@@ -23,22 +21,22 @@ Reserved Notation "t1 '↪' t2" (at level 60, t1 constr, t2 constr).
 
 Inductive step : tm -> tm -> Prop :=
 | STEffOp: forall op (c1 c: constant) e,
-    body e -> lc c1 -> lc c ->
-    ⇓{op ~ c1}{c} -> (tleteffop op c1 e) ↪ (e ^t^ c)
+    body e -> lc (vconst c1) -> lc (vconst c) ->
+    ⇓{op ~ c1}{c} -> (tleteffop op c1 e) ↪ (e ^^ (vconst c))
 | STLetE1: forall e1 e1' e,
     body e ->
     e1 ↪ e1' ->
     (tlete e1 e) ↪ (tlete e1' e)
 | STLetE2: forall (v1: value) e,
     lc v1 -> body e ->
-    (tlete (treturn v1) e) ↪ (e ^t^ v1)
+    (tlete (treturn v1) e) ↪ (e ^^ v1)
 | STLetAppLam: forall T (v_x: value) e1 e,
     body e1 -> body e -> lc v_x ->
-    (tletapp (vlam T e1) v_x e) ↪ tlete (e1 ^t^ v_x) e
+    (tletapp (vlam T e1) v_x e) ↪ tlete (e1 ^^ v_x) e
 | STLetAppFix: forall T_f (v_x: value) (e1: tm) e,
     body (vlam T_f e1) -> lc v_x -> body e ->
-    tletapp (vfix T_f (vlam T_f e1)) v_x e ↪
-      tletapp ((vlam T_f e1) ^v^ v_x) (vfix T_f (vlam T_f e1)) e
+    tletapp (vfix T_f (treturn (vlam T_f e1))) v_x e ↪
+      tletapp ((vlam T_f e1) ^^ v_x) (vfix T_f (treturn (vlam T_f e1))) e
 | STMatchbTrue: forall e1 e2,
     lc e1 -> lc e2 ->
     (tmatchb true e1 e2) ↪ e1
@@ -61,32 +59,46 @@ Global Hint Constructors multistep : core.
 
 (** * Properties of operational semantics *)
 
+Lemma body_vbvar: forall bn, body (vbvar bn) <-> bn = 0.
+Proof.
+  split; intros.
+  - invclear H. auto_pose_fv y. specialize_with y. ln_simpl; eauto.
+    inversion H0.
+  - hauto. 
+Qed.
+
+Ltac lc_solver_aux2 :=
+  match goal with
+  | [H: lc (treturn ?v) |- lc ?v ] => sinvert H; auto
+  | [H: lc ?v |- lc (treturn ?v) ] => econstructor; eauto
+  | [H: body (vlam _ _) |- _ ] => rewrite body_abs_iff_body2 in H; mydestr; auto
+  | [H: body2 ?e |- body (vlam _ ?e) ] => rewrite body_abs_iff_body2; auto
+  | [H: body2 ?e |- body ({1 ~> ?u} ?e) ] => apply open_body; auto
+  | [H: body ?e |- lc ({0 ~> ?u} ?e) ] => apply open_lc; auto
+  | [H: body (vbvar _) |- _ ] => rewrite body_vbvar in H; subst; auto
+  | [ |- body (vbvar _) ] => apply body_vbvar; auto
+  | [H: lc ?e |- lc ({?i ~> ?u} ?e) ] => rewrite open_rec_lc; auto
+  | _ => lc_solver_aux1
+  end.
+
+Ltac lc_solver:= 
+autounfold with class_simpl; simpl; mydestr; auto; fold_syntax_class;
+repeat (lc_solver_aux2; auto); fold_syntax_class.
+
 Lemma step_regular: forall e1 e2, e1 ↪ e2 -> lc e1 /\ lc e2.
 Proof.
   intros.
-  induction H; split; auto.
-  - destruct H. econstructor; auto. apply H.
-  - apply open_lc_tm; auto.
-  - destruct_hyp_conj. rewrite lete_lc_body; split; auto.
-  - destruct_hyp_conj. rewrite lete_lc_body; split; auto.
-  - try destruct_hyp_conj. rewrite lete_lc_body; split; auto.
-  - apply open_lc_tm; auto.
-  - rewrite letapp_lc_body; split; auto. rewrite lc_abs_iff_body; auto.
-  - rewrite lete_lc_body; split; auto. apply open_lc_tm; auto.
-  - rewrite letapp_lc_body; split; auto. rewrite lc_fix_iff_body; auto.
-  - rewrite letapp_lc_body; split; auto.
-    + eapply open_lc_value; eauto.
-    + rewrite body_vlam_eq in H. rewrite lc_fix_iff_body; eauto.
+  induction H; split; auto; lc_solver.
 Qed.
 
 Lemma step_regular1: forall e1 e2, e1 ↪ e2 -> lc e1.
 Proof.
-  intros. apply step_regular in H. destruct H; auto.
+  intros. apply step_regular in H. hauto.
 Qed.
 
 Lemma step_regular2: forall e1 e2, e1 ↪ e2 -> lc e2.
 Proof.
-  intros. apply step_regular in H. destruct H; auto.
+  intros. apply step_regular in H. hauto.
 Qed.
 
 Global Hint Resolve step_regular1: core.
@@ -95,13 +107,12 @@ Global Hint Resolve step_regular2: core.
 Theorem multistep_trans: forall (x y z : tm), x ↪* y -> y ↪* z -> x ↪* z.
 Proof.
   intros. generalize dependent z.
-  induction H; intros; eauto.
+  induction H; eauto.
 Qed.
 
 Theorem multistep_R : forall (x y : tm),
     x ↪ y -> x ↪* y.
-Proof. intros. eauto.
-Qed.
+Proof. eauto. Qed.
 
 Lemma multi_step_regular: forall e1 e2, e1 ↪* e2 -> lc e1 /\ lc e2.
 Proof.
@@ -118,27 +129,13 @@ Proof.
   intros. apply multi_step_regular in H. destruct H; auto.
 Qed.
 
-Ltac step_regular_simp :=
-  repeat match goal with
-    | [H: _ ↪* _ |- lc _ ] => apply multi_step_regular in H; destruct H; auto
-    | [H: _ ↪ _ |- lc _ ] => apply step_regular in H; destruct H; auto
-    | [H: _ ↪* _ |- body _] => apply multi_step_regular in H; destruct H; auto
-    | [H: _ ↪ _ |- body _] => apply step_regular in H; destruct H; auto
-    end.
-
-Lemma value_reduction_refl: forall (v1: value) v2, v1 ↪* v2 -> v2 = v1.
+Lemma value_reduction_refl: forall (v1: value) v2, (treturn v1) ↪* (treturn v2) -> v2 = v1.
 Proof.
   intros * H. sinvert H; easy.
 Qed.
 
-Ltac reduction_simp :=
-  match goal with
-  | H: (treturn _) ↪* _  |- _ =>
-      apply value_reduction_refl in H; simp_hyps; simplify_eq
-  end.
-
 Lemma reduction_tlete:  forall e_x e (v : value),
-    tlete e_x e ↪* v -> (exists (v_x: value), e_x ↪* v_x /\ (e ^t^ v_x) ↪* v).
+    tlete e_x e ↪* (treturn v) -> (exists (v_x: value), e_x ↪* (treturn v_x) /\ (e ^^ v_x) ↪* (treturn v)).
 Proof.
   intros.
   remember (tlete e_x e). remember (treturn v).
@@ -147,7 +144,7 @@ Proof.
   sinvert H.
   - ospecialize* IHmultistep; eauto.
     simp_hyps. repeat esplit; eauto.
-  - repeat esplit. econstructor; eauto. eauto.
+  - repeat esplit. econstructor; eauto. lc_solver. eauto.
 Qed.
 
 Lemma reduction_tlete':  forall e_x e (v_x v : value),
@@ -155,13 +152,13 @@ Lemma reduction_tlete':  forall e_x e (v_x v : value),
     regularity lemma. Remove later when we bother proving a few more naming
     lemmas. *)
     body e ->
-    e_x ↪* v_x ->
-    (e ^t^ v_x) ↪* v ->
-    tlete e_x e ↪* v.
+    e_x ↪* (treturn v_x) ->
+    (e ^^ v_x) ↪* (treturn v) ->
+    tlete e_x e ↪* (treturn v).
 Proof.
   intros * Hb H. remember (treturn v_x).
   induction H; intros; subst.
-  - econstructor; eauto using STLetE2.
+  - lc_solver. econstructor; eauto using STLetE2.
   - simp_hyps.
     simplify_list_eq.
     econstructor.
@@ -171,9 +168,9 @@ Qed.
 
 Lemma reduction_tlete_iff:
   ∀ (e_x e : tm) (v : value),
-    tlete e_x e ↪* v
+    tlete e_x e ↪* (treturn v)
     <-> (body e /\ ∃ (v_x : value),
-          e_x ↪* v_x ∧ e ^t^ v_x ↪* v).
+          e_x ↪* (treturn v_x) ∧ e ^^ v_x ↪* (treturn v)).
 Proof.
   split.
   - split. apply multi_step_regular in H. simp_hyps. lc_solver.
@@ -183,36 +180,36 @@ Qed.
 
 Lemma reduction_mk_app_v_v (f v_x v : value) :
   lc v_x ->
-  mk_app f v_x ↪* v ->
-  tletapp f v_x (vbvar 0) ↪* v.
+  mk_app (treturn f) (treturn v_x) ↪* (treturn v) ->
+  tletapp f v_x (treturn (vbvar 0)) ↪* (treturn v).
 Proof.
   intros Hlc H.
   sinvert H. sinvert H0. easy.
   sinvert H1. sinvert H. easy.
-  simpl in *. simplify_list_eq.
-  repeat rewrite open_rec_lc_value in * by eauto.
-  eauto.
+  ln_simpl. 
+  repeat rewrite open_rec_lc in * by eauto. eauto.
 Qed.
 
-Lemma body_mk_app_aux2 (f: value): lc f -> body (tletapp f (vbvar 0) (vbvar 0)).
+Lemma body_mk_app_aux2 (f: value): lc f -> body (tletapp f (vbvar 0) (treturn (vbvar 0))).
 Proof.
-  eexists. instantiate_atom_listctx.
-  simpl. apply letapp_lc_body. repeat split; eauto using lc.
-  by rewrite open_rec_lc_value.
+  intros Hlc. auto_exists_L. intros x Hx.
+  ln_simpl.
+  apply letapp_lc_body. repeat split; lc_solver. 
 Qed.
 
 Lemma body_mk_app_aux v_x:
   lc v_x ->
-  body (tlete v_x (tletapp (vbvar 1) (vbvar 0) (vbvar 0))).
+  body (tlete v_x (tletapp (vbvar 1) (vbvar 0) (treturn (vbvar 0)))).
 Proof.
-  eexists. instantiate_atom_listctx.
-  simpl. apply lete_lc_body. repeat split; eauto using lc.
-  by rewrite open_rec_lc_tm.
+  intros Hlc. auto_exists_L. intros x Hx.
+  ln_simpl.
+  apply lete_lc_body. repeat split; lc_solver.
+  apply body_mk_app_aux2; lc_solver.
 Qed.
 
 Lemma reduction_mk_app_v_v' (f v_x v : value) :
-  tletapp f v_x (vbvar 0) ↪* v ->
-  mk_app f v_x ↪* v.
+  tletapp f v_x (treturn (vbvar 0)) ↪* (treturn v) ->
+  mk_app (treturn f) (treturn v_x) ↪* (treturn v).
 Proof.
   intros H.
   assert (lc v_x). {
@@ -222,38 +219,36 @@ Proof.
     apply multi_step_regular1 in H. sinvert H. eauto.
   }
   eapply_eq multistep_step.
-  eapply STLetE2.
-  - apply multi_step_regular1 in H. sinvert H. eauto.
-  (* Probably should be a lemma. *)
-  - apply body_mk_app_aux; eauto.
-  - simpl. simplify_list_eq. rewrite open_rec_lc_value; eauto.
+  eapply STLetE2; eauto.
+  - apply body_mk_app_aux; eauto. lc_solver.
+  - ln_simpl. rewrite open_rec_lc; eauto.
     eapply_eq multistep_step.
     eapply STLetE2; eauto.
-    simpl. by rewrite open_rec_lc_value.
+    ln_simpl. by rewrite open_rec_lc.
 Qed.
 
-Lemma open_vlam_rev k Tb e (v: value): vlam Tb ({S k ~t> v} e) = {k ~v> v} vlam Tb e.
+Lemma open_vlam_rev k Tb e (v: value): vlam Tb ({S k ~> v} e) = {k ~> v} (vlam Tb e).
 Proof. eauto. Qed.
 
 Lemma reduction_mk_app_lam Tb e (v_x : value) (v : value) :
   lc v_x ->
-  mk_app (vlam Tb e) v_x ↪* v ->
-  e ^t^ v_x ↪* v.
+  mk_app (treturn (vlam Tb e)) (treturn v_x) ↪* (treturn v) ->
+  (e ^^ v_x) ↪* (treturn v).
 Proof.
   unfold mk_app. intros Hlc H.
   assert (lc (vlam Tb e)) as Haux. {
-    step_regular_simp. sinvert H; eauto.
+    apply multi_step_regular1 in H. sinvert H. lc_solver. 
   }
-  apply reduction_tlete in H. simp_hyps. simpl in *.
-  rewrite open_rec_lc_value in H1; eauto.
+  apply reduction_tlete in H. simp_hyps. ln_simpl.
+  rewrite open_rec_lc in H1; eauto.
   apply value_reduction_refl in H0; sinvert H0.
-  apply reduction_tlete in H1. simp_hyps. simpl in *.
-  rewrite open_vlam_rev in H1.
-  rewrite open_rec_lc_value in H1; eauto.
-  apply value_reduction_refl in H0; sinvert H0.
-  sinvert H1. sinvert H.
-  apply reduction_tlete in H0.
-  simp_hyps. simpl in *.
+  apply reduction_tlete in H1. simp_hyps. ln_simpl.
+  apply value_reduction_refl in H1; sinvert H1.
+  rewrite open_vlam_rev in H2.
+  rewrite open_rec_lc in H2; eauto.
+  sinvert H2. sinvert H0.
+  apply reduction_tlete in H1.
+  simp_hyps. ln_simpl.
   eapply multistep_trans; eauto.
 Qed.
 
@@ -262,30 +257,27 @@ Lemma reduction_mk_app_lam' Tb e (v_x : value) (v : value) :
   (* NOTE: This condition is unnecessary as it should be implied by the
   regularity lemma. *)
   body e ->
-  e ^t^ v_x ↪* v ->
-  mk_app (vlam Tb e) v_x ↪* v.
+  e ^^ v_x ↪* (treturn v) ->
+  mk_app (treturn (vlam Tb e)) (treturn v_x) ↪* (treturn v).
 Proof.
   unfold mk_app. intros Hlc Hb H.
+  assert (lc (treturn v_x)) as Hlc_tm by lc_solver.
   assert (lc (vlam Tb e)) as Haux by lc_solver.
+  assert (lc (treturn (vlam Tb e))) as Haux_tm by lc_solver.
+  assert (lc v) as Hlc_v. { apply multi_step_regular in H. lc_solver. }
+  assert (lc (treturn v)) as Hlc_v_tm by lc_solver.
   apply reduction_tlete' with (v_x := vlam Tb e); eauto.
-  apply body_mk_app_aux; eauto.
-  simpl. rewrite open_rec_lc_value; eauto.
+  apply body_mk_app_aux; lc_solver.
+  ln_simpl. rewrite open_rec_lc; eauto.
   apply reduction_tlete' with (v_x := v_x); eauto.
-  simpl. rewrite open_vlam_rev; rewrite open_rec_lc_value; eauto.
-  eapply_eq multistep_step. econstructor; eauto.
-  apply reduction_tlete' with (v_x := v); eauto.
-  simpl. econstructor. eauto using multi_step_regular2.
+  ln_simpl. rewrite open_vlam_rev; rewrite open_rec_lc; eauto.
+  eapply_eq multistep_step. econstructor; eauto. lc_solver.
+  apply reduction_tlete' with (v_x := v); eauto. lc_solver.
 Qed.
 
-Ltac value_reduction_simp :=
-  repeat
-    match goal with
-    | [H: treturn _ ↪* treturn _ |- _ ] => apply value_reduction_refl in H; sinvert H
-    end.
-
 Lemma reduction_tletapp:  forall v1 v2 e (v : value),
-    tletapp v1 v2 e ↪* v ->
-    (exists (v_x: value), tletapp v1 v2 (vbvar 0) ↪* v_x /\ (e ^t^ v_x) ↪* v).
+    tletapp v1 v2 e ↪* (treturn v) ->
+    (exists (v_x: value), tletapp v1 v2 (treturn (vbvar 0)) ↪* (treturn v_x) /\ (e ^^ v_x) ↪* (treturn v)).
 Proof.
   intros.
   remember (tletapp v1 v2 e). remember (treturn v).
@@ -294,42 +286,41 @@ Proof.
   induction H; intros; subst. easy.
   simp_hyps. sinvert H.
   - eapply reduction_tlete in H0. simp_hyps.
+    assert (lc (treturn v_x)) as Hlc_tm by solve [apply multi_step_regular2 in H0; eauto].
     simplify_list_eq.
     eexists _. repeat split; eauto using reduction_mk_app_lam'.
-    eapply_eq multistep_step. econstructor; eauto.
-    eapply reduction_tlete'; eauto. simpl.
-    econstructor. apply multi_step_regular2 in H0; eauto.
+    eapply_eq multistep_step. econstructor; eauto. lc_solver.
+    eapply reduction_tlete'; eauto. lc_solver.
   - simplify_list_eq.
     ospecialize* H1; eauto. simp_hyps.
     eexists _.
     repeat split; cycle 1; eauto.
-    eapply_eq multistep_step. econstructor; eauto.
-    simpl. eauto.
+    eapply_eq multistep_step. econstructor; eauto. lc_solver.
+    ln_simpl. eauto.
 Qed.
 
 Lemma reduction_tletapp':  forall v1 v2 e (v : value),
-    (body e /\ exists (v_x: value), tletapp v1 v2 (vbvar 0) ↪* v_x /\ (e ^t^ v_x) ↪* v) -> tletapp v1 v2 e ↪* v.
+    (body e /\ exists (v_x: value), tletapp v1 v2 (treturn (vbvar 0)) ↪* (treturn v_x) /\ (e ^^ v_x) ↪* (treturn v)) -> tletapp v1 v2 e ↪* (treturn v).
 Proof.
   intros. destruct H as (He & (v_x & Hv_x & H)).
-  remember (tletapp v1 v2 (vbvar 0)). remember (treturn v_x).
+  remember (tletapp v1 v2 (treturn (vbvar 0))). remember (treturn v_x).
   generalize dependent v2.
   generalize dependent v1.
   generalize dependent v_x.
   induction Hv_x; intros; subst. easy.
   simp_hyps. sinvert H.
   - clear IHHv_x.
-    eapply reduction_tlete in Hv_x. simp_hyps.
-    simplify_list_eq. value_reduction_simp.
+    eapply reduction_tlete in Hv_x. simp_hyps. ln_simpl.
+    apply value_reduction_refl in H2; invclear H2. clear H.
     eapply_eq multistep_step. econstructor; eauto.
     eapply reduction_tlete'; eauto.
-  - simplify_list_eq.
-    ospecialize* IHHv_x; eauto.
+  - ospecialize* IHHv_x; eauto.
     eapply_eq multistep_step. econstructor; eauto.
-    simpl. eauto.
+    ln_simpl. eauto.
 Qed.
 
 Lemma reduction_tletapp_iff:  forall v1 v2 e (v : value),
-    tletapp v1 v2 e ↪* v <-> (body e /\ exists (v_x: value), tletapp v1 v2 (vbvar 0) ↪* v_x /\ (e ^t^ v_x) ↪* v).
+    tletapp v1 v2 e ↪* (treturn v) <-> (body e /\ exists (v_x: value), tletapp v1 v2 (treturn (vbvar 0)) ↪* (treturn v_x) /\ (e ^^ v_x) ↪* (treturn v)).
 Proof.
   split; intros.
   - split. apply multi_step_regular1 in H. lc_solver.
@@ -337,26 +328,25 @@ Proof.
   - apply reduction_tletapp'; eauto.
 Qed.
 
-Lemma value_reduction_any_ctx: forall (v1: value), lc v1 -> v1 ↪* v1.
+Lemma value_reduction_any_ctx: forall (v1: value), lc v1 -> (treturn v1) ↪* (treturn v1).
 Proof.
-  intros. econstructor; eauto.
+  intros. econstructor; eauto. lc_solver.
 Qed.
 
 Lemma reduction_tleteffop:  forall op v2 e (v : value),
-    (tleteffop op v2 e) ↪* v ->
+    (tleteffop op v2 e) ↪* (treturn v) ->
     exists (c2 c_x: constant),
-      v2 = c2 /\ ⇓{op ~ c2}{ c_x } /\ (e ^t^ c_x) ↪* v.
+      v2 = c2 /\ ⇓{op ~ c2}{ c_x } /\ (e ^^ (vconst c_x)) ↪* (treturn v).
 Proof.
   intros.
   sinvert H. sinvert H0.
   eauto 10.
 Qed.
 
-
 Lemma reduction_tleteffop_iff:  forall op v2 e (v : value),
-    (tleteffop op v2 e) ↪* v <->
+    (tleteffop op v2 e) ↪* (treturn v) <->
       body e /\ exists (c2 c_x: constant),
-        v2 = c2 /\ ⇓{op ~ c2}{ c_x } /\ (e ^t^ c_x) ↪* v.
+        v2 = c2 /\ ⇓{op ~ c2}{ c_x } /\ (e ^^ (vconst c_x)) ↪* (treturn v).
 Proof.
   split.
   - intuition.
@@ -366,7 +356,7 @@ Proof.
 Qed.
 
 Lemma reduction_matchb_true:  forall e1 e2 (v : value),
-    tmatchb true e1 e2 ↪* v -> e1 ↪* v.
+    tmatchb true e1 e2 ↪* (treturn v) -> e1 ↪* (treturn v).
 Proof.
   intros.
   sinvert H.
@@ -374,36 +364,54 @@ Proof.
 Qed.
 
 Lemma reduction_matchb_false:  forall e1 e2 (v : value),
-    tmatchb false e1 e2 ↪* v -> e2 ↪* v.
+    tmatchb false e1 e2 ↪* (treturn v) -> e2 ↪* (treturn v).
 Proof.
   intros.
   sinvert H.
   sinvert H0. simplify_list_eq. eauto.
 Qed.
 
+Ltac step_regular_simp :=
+  repeat match goal with
+    | [H: _ ↪* _ |- _ ] =>
+      first
+        [ lazymatch goal with
+          | |- lc _ => idtac
+          | |- body _ => idtac
+          | |- body2 _ => idtac
+          end;
+          apply multi_step_regular in H; destruct H; auto
+        | fail 1 ]
+    | [H: _ ↪ _ |- _ ] =>
+      first
+        [ lazymatch goal with
+          | |- lc _ => idtac
+          | |- body _ => idtac
+          | |- body2 _ => idtac
+          end;
+          apply step_regular in H; destruct H; auto
+        | fail 1 ]
+    | H: (treturn _) ↪* (treturn _)  |- _ =>
+      apply value_reduction_refl in H; simp_hyps; simplify_eq
+    | [|- ?e ↪ ?e ] => econstructor; eauto
+    end.
+
 (** NOTE: reduction lemmas for underapproximation *)
 
-Ltac lc_solver_simp_aux :=
-  match goal with
-  | [H: _ ↪* _ |- lc _] => apply multi_step_regular in H; simp_hyps
-  | [H: _ ↪* _ |- body _] => apply multi_step_regular in H; simp_hyps
-  end.
-
-Ltac lc_solver_simp :=
-  repeat lc_solver_simp_aux; eauto.
-
-Ltac lc_solver_plus_aux :=
+Ltac lc_solver_aux3 :=
   match goal with
   | [H: lc (tlete _ _) |- lc _] => rewrite lete_lc_body in H; simp_hyps
   | [H: lc (tlete _ _) |- body _] => rewrite lete_lc_body in H; simp_hyps
+  | _ => lc_solver_aux2
   end.
 
-Ltac lc_solver_plus :=
-  eauto; lc_solver_simp; eauto;
-  (repeat lc_solver_plus_aux); eauto.
+Ltac lc_solver3 :=
+  ln_simpl;
+  step_regular_simp; eauto;
+  repeat (lc_solver_aux3; auto); fold_syntax_class.
 
-Lemma reduction_tlete_value: forall (v1: value) e2,
-  forall (v: value), tlete v1 e2 ↪* v <-> (lc v1 /\ body e2 /\ e2 ^t^ v1 ↪* v).
+(* Lemma reduction_tlete: forall (v1: value) e2,
+  forall (v: value), tlete v1 e2 ↪* v <-> (lc v1 /\ body e2 /\ e2 ^^ v1 ↪* v).
 Proof.
   split; intros.
   - assert (lc v1) by lc_solver_plus.
@@ -411,27 +419,23 @@ Proof.
     apply reduction_tlete in H. simp_hyps.
     apply value_reduction_refl in H2. simp_hyps. subst; intuition.
   - simp_hyps. eapply reduction_tlete'; eauto.
-Qed.
+Qed. *)
 
 Lemma reduction_nest_tlete: forall e,
-  forall (v: value), tlete e (vbvar 0) ↪* v <-> e ↪* v.
+  forall (v: value), tlete e (treturn (vbvar 0)) ↪* (treturn v) <-> e ↪* (treturn v).
 Proof.
   intros e. split; intros.
-  - apply reduction_tlete in H. simp_hyps. simpl in *.
-    apply value_reduction_refl in H1.
-    simp_hyps. subst. eauto.
-  - eapply reduction_tlete'; eauto. simpl.
-    apply (value_reduction_any_ctx v); eauto.
-    apply multi_step_regular2 in H; eauto.
+  - apply reduction_tlete in H. lc_solver3.
+  - eapply reduction_tlete'; lc_solver3.
+    econstructor. lc_solver3.
 Qed.
 
 Lemma reduction_tletapp_lam:  forall T e1 v2 e (v : value),
-    tletapp (vlam T e1) v2 e ↪* v <->
-      (lc v2 /\ lc (vlam T e1) /\ tlete (e1 ^t^ v2) e ↪* v).
+    tletapp (vlam T e1) v2 e ↪* (treturn v) <->
+      (lc v2 /\ lc (vlam T e1) /\ tlete (e1 ^^ v2) e ↪* (treturn v)).
 Proof.
   split; intros.
-  - inversion H; subst. inversion H0; subst; eauto.
-    intuition; eauto. lc_solver.
+  - invclear H. invclear H0. repeat split; lc_solver3.
   - simp_hyps. eapply_eq multistep_step; eauto.
     apply multi_step_regular1 in H2; eauto.
     rewrite lete_lc_body in H2; simp_hyps; eauto.
@@ -439,12 +443,11 @@ Proof.
 Qed.
 
 Lemma reduction_tletapp_fix:  forall T_f (v_x: value) (e1: tm) e (v : value),
-      tletapp (vfix T_f (vlam T_f e1)) v_x e ↪* v <->
-        (lc v_x /\ tletapp ((vlam T_f e1) ^v^ v_x) (vfix T_f (vlam T_f e1)) e ↪* v).
+      tletapp (vfix T_f (treturn (vlam T_f e1))) v_x e ↪* (treturn v) <->
+        (lc v_x /\ tletapp ((vlam T_f e1) ^^ v_x) (vfix T_f (treturn (vlam T_f e1))) e ↪* (treturn v)).
 Proof.
   split; intros.
   - inversion H; subst. inversion H0; subst; eauto.
-    (* intuition; eauto. lc_solver. *)
   - simp_hyps. eapply_eq multistep_step; eauto.
     apply multi_step_regular in H0; simp_hyps; eauto.
     econstructor; eauto. rewrite letapp_lc_body in H0. simp_hyps.
@@ -453,21 +456,21 @@ Qed.
 
 Lemma reduction_mk_app_iff:  forall e e_x (v : value),
     lc e_x ->
-    mk_app e e_x ↪* v <->
-      (exists (f v_x: value), e ↪* f /\ e_x ↪* v_x /\ tletapp f v_x (vbvar 0) ↪* v).
+    mk_app e e_x ↪* (treturn v) <->
+      (exists (f v_x: value), e ↪* (treturn f) /\ e_x ↪* (treturn v_x) /\ tletapp f v_x (treturn (vbvar 0)) ↪* (treturn v)).
 Proof.
   intros e e_x v Hlc.
   unfold mk_app.
   split; intros.
   - apply reduction_tlete in H. destruct H as (f & Hf & H).
-    simpl in H. rewrite open_rec_lc_tm in H by eauto.
+    ln_simpl. rewrite open_rec_lc in H by eauto.
     apply reduction_tlete in H. destruct H as (v_x & Hv_x & H).
-    simpl in H. rewrite open_rec_lc_value in H by lc_solver_plus.
+    ln_simpl. rewrite open_rec_lc in H by lc_solver3.
     exists f, v_x. intuition.
   - destruct H as (f & v_x & Hf & Hv_x & H).
     eapply reduction_tlete'; eauto. apply body_mk_app_aux; eauto.
-    simpl. rewrite open_rec_lc_tm; eauto.
-    eapply reduction_tlete'; eauto. apply body_mk_app_aux2. by lc_solver_plus.
-    simpl. rewrite open_rec_lc_value; eauto.
-    all: by lc_solver_plus.
+    ln_simpl. rewrite open_rec_lc; eauto.
+    eapply reduction_tlete'; eauto. apply body_mk_app_aux2. by lc_solver3.
+    ln_simpl. rewrite open_rec_lc; eauto.
+    lc_solver3.
 Qed.
