Syntax/BasicTyping.v
@@ -7,40 +7,40 @@ Import BaseDef.
 Import Lang.
 Import Primitives.
 
-Definition context := amap ty.
+Definition tyctx := amap ty.
 #[global]
-Instance context_stale : Stale context := dom.
-Arguments context_stale /.
+Instance tyctx_stale : Stale tyctx := dom.
+Arguments tyctx_stale /.
 
 (** Basic typing rules  *)
-Inductive tm_has_type : context -> tm -> ty -> Prop :=
+Inductive tm_has_type : tyctx -> tm -> ty -> Prop :=
 | BtErr: forall Γ T, tm_has_type Γ (terr T) T
 | BtValue : forall Γ v T, value_has_type Γ v T -> tm_has_type Γ (treturn v) T
 | BtLetE : forall Γ e1 e2 T1 T2 (L: aset),
     tm_has_type Γ e1 T1 ->
-    (forall (x: atom), x ∉ L -> tm_has_type (<[ x := T1]> Γ) (e2 ^^ x) T2) ->
+    (forall (x: atom), x ∉ L -> tm_has_type (<[ x := T1]> Γ) (e2 ^^ (vfvar x)) T2) ->
     tm_has_type Γ (tlete e1 e2) T2
 | BtEffOp : forall Γ (op: effop) v1 e (T1 Tx: base_ty) T (L: aset),
     value_has_type Γ v1 T1 ->
     (ty_of_op op) = T1 ⤍ Tx ->
-    (forall (x: atom), x ∉ L -> tm_has_type (<[x := TBase Tx]> Γ) (e ^^ x) T) ->
+    (forall (x: atom), x ∉ L -> tm_has_type (<[x := TBase Tx]> Γ) (e ^^ (vfvar x)) T) ->
     tm_has_type Γ (tleteffop op v1 e) T
 | BtApp : forall Γ v1 v2 e T1 Tx T (L: aset),
     value_has_type Γ v1 (T1 ⤍ Tx) ->
     value_has_type Γ v2 T1 ->
-    (forall (x: atom), x ∉ L -> tm_has_type (<[x := Tx]> Γ) (e ^^ x) T) ->
+    (forall (x: atom), x ∉ L -> tm_has_type (<[x := Tx]> Γ) (e ^^ (vfvar x)) T) ->
     tm_has_type Γ (tletapp v1 v2 e) T
 | BtMatchb: forall Γ v e1 e2 T,
     value_has_type Γ v TBool ->
     tm_has_type Γ e1 T ->
     tm_has_type Γ e2 T ->
     tm_has_type Γ (tmatchb v e1 e2) T
-with value_has_type : context -> value -> ty -> Prop :=
+with value_has_type : tyctx -> value -> ty -> Prop :=
 | BtConst : forall Γ (c: constant), value_has_type Γ (vconst c) (ty_of_const c)
 | BtVar : forall Γ (x: atom) T,
     Γ !! x = Some T -> value_has_type Γ (vfvar x) T
 | BtFun : forall Γ Tx T e (L: aset),
-    (forall (x: atom), x ∉ L -> tm_has_type (<[x := Tx]> Γ) (e ^^ x) T) ->
+    (forall (x: atom), x ∉ L -> tm_has_type (<[x := Tx]> Γ) (e ^^ (vfvar x)) T) ->
     value_has_type Γ (vlam Tx e) (Tx ⤍ T)
 | BtFix : forall Γ (Tx: base_ty) T e (L: aset),
     (forall (x: atom), x ∉ L -> value_has_type (<[x := TBase Tx]>Γ) (vlam (Tx ⤍ T) e ^^ (vfvar x)) ((Tx ⤍ T) ⤍ T)) ->
@@ -53,9 +53,9 @@ Global Hint Constructors tm_has_type: core.
 Global Hint Constructors value_has_type: core.
 
 #[global]
-Instance has_normal_type_tm_instance : Typing context tm ty := tm_has_type.
+Instance has_normal_type_tm_instance : Typing tyctx tm ty := tm_has_type.
 Arguments has_normal_type_tm_instance /.
 
 #[global]
-Instance has_normal_type_value_instance : Typing context value ty := value_has_type.
+Instance has_normal_type_value_instance : Typing tyctx value ty := value_has_type.
 Arguments has_normal_type_value_instance /.
