LocallyNameless/Lc.v
@@ -1,0 +1,61 @@
+From CT.LocallyNameless Require Export FineRty LangLc QualifierLc RtyLc.
+
+Import BaseDef MyTactics Primitives Lang LangLc Syntax.
+
+(* There are some more lemmas for better lc solver. *)
+
+Lemma body_abs_iff_body2: forall T e, body (vlam T e) <-> body2 e.
+Proof.
+  split; unfold body; unfold body2; intros.
+  - mydestr. 
+    auto_exists_L. intros y Hy. specialize_with y.
+    intros z Hz.
+    ln_simpl; eauto.
+    rewrite -> lc_abs_iff_body in H; eauto.
+    apply open_lc; eauto. lc_solver1.
+  - mydestr.
+    auto_exists_L; intros y Hy. specialize_with y.
+    ln_simpl; eauto.
+    rewrite -> lc_abs_iff_body; eauto.
+    auto_exists_L; eauto.
+Qed.
+
+Class OpenBody A `{Stale A} `{Open value A} `{Lc A} := open_body :
+forall (e: A) (u: value), body2 e -> lc u -> body ({1 ~> u} e).
+
+Lemma OpenBody_all
+  (A : Type)
+  (staleA : Stale A)
+  (openA  : Open value A)
+  (substA : Subst value A)
+  (lcA    : Lc A)
+  (substIntroA : @SubstIntro A staleA openA substA lcA)
+  (substBodyA    : @SubstBody A staleA openA substA lcA)
+  : @OpenBody A staleA openA lcA.
+Proof.
+  intros e u Hbody Hlc. destruct Hbody as [L Hbody].
+  pose_fresh_fv y. specialize_with y.
+  erewrite <- subst_intro; auto. instantiate (1:= y).
+  eapply subst_body; eauto. 
+  auto_exists_L; intros z Hz. my_set_solver.
+Qed.
+
+#[global] Instance OpenBody_tm : OpenBody tm.
+Proof. apply OpenBody_all with (staleA := stale) (openA := open) (substA := subst) (lcA := lc); typeclasses eauto. Qed.
+Arguments OpenBody_tm /.
+
+#[global] Instance OpenBody_value : OpenBody value.
+Proof. apply OpenBody_all with (staleA := stale) (openA := open) (substA := subst) (lcA := lc); typeclasses eauto. Qed.
+Arguments OpenBody_value /.
+
+Ltac lc_solver_aux2 :=
+  match goal with
+  | [H: body (vlam _ _) |- _ ] => rewrite body_abs_iff_body2 in H; mydestr; auto
+  | [H: body2 ?e |- body (vlam _ ?e) ] => rewrite body_abs_iff_body2; auto
+  | [H: body2 ?e |- body ({1 ~> ?u} ?e) ] => apply open_body; auto
+  | _ => lc_solver_aux1
+  end.
+
+Ltac lc_solver:= 
+autounfold with class_simpl; simpl; mydestr; auto; fold_syntax_class;
+repeat (lc_solver_aux2; auto); fold_syntax_class.
